\documentclass{article}
\usepackage[utf8]{inputenc}
\usepackage{amsmath}
\usepackage{amssymb}
\usepackage{physics}
\usepackage{gensymb}
\usepackage{esvect}
\usepackage[title]{appendix} % or other options
\usepackage{graphicx} % Required for inserting images


\title{Personal solutions to GR book by Carroll chapter 1}
\author{Baset}
\date{June 2025}

\begin{document}
\author{Baset}
\maketitle
\section*{1.}
Let the initial velocity of the particle with respect to the obesrver $S'$ be $u_0' \stackrel{S'}{\equiv} (u_0^{x'}, u_0^{y'})$.
For simplicity, we assume that the collision happens at $t' = 0$. Moreover, we assume observers $S$ and $S'$ are aligned along the $x$-axis and that when $t'=0$ then 
$t = 0$. Let at $t'=0$ the line that describes the mirror be $-x' = y'$. The line that describes the particle is $\frac{x'}{u_0^{x'}} = \frac{y'}{u_0^{y'}}$. For now, 
$u_0^{x'}, u_0^{y'} \ne 0$. Now, we will find the angle between these two lines:
\begin{equation}
    \tan \theta' = |\frac{\tan{\frac{\pi}{4}} - \frac{u_0^{y'}}{u_0^{x'}}}{1 + \tan{\frac{\pi}{4}} \frac{u_0^{y'}}{u_0^{x'}}}| = |\frac{1 - \frac{u_0^{y'}}{u_0^{x'}}}{1 + \frac{u_0^{y'}}{u_0^{x'}}} |
\end{equation}
We let the $u_0^{y'} = u_0^{x'}\tan{\alpha'} = u_0^{x}\tan{\alpha'}$. Then, we have that:
\begin{equation}
    \tan \theta' = |\frac{1 - \tan{\alpha'}}{1 + \tan{\alpha'}}|
\end{equation}
But in the frame $S$, we have that the $u_0^{y} = \frac{u_0^{y'}+v}{1+u_0^{y'}v}$. Also, the mirror's coordinates in $S$ are:
\begin{equation}
    y = \gamma(y' + vt') = \gamma y'|_{t'=0}
\end{equation}
Therefore, w.r.t. to $S$ at $t=0$ the mirror is $y = -\frac{x}{\gamma}$. The particle's coordinates in $S$ are $y = 
\frac{u_0^{y'}+v}{(1+u_0^{y'}v)u_0^{x}}x$. Therefore, the angle between the particle and the mirror is:
\begin{equation}
    \tan \theta = |\frac{\gamma - \frac{u_0^{y'}+v}{(1+u_0^{y'}v)u_0^{x}}}{1 + \gamma \frac{u_0^{y'}+v}{(1+u_0^{y'}v)u_0^{x}}}| \implies
    \tan \theta = |\frac{\gamma - \frac{\tan{\alpha'}+ v/u_0^{x}}{1+\tan{\alpha'}u_0^{x}v}}{1 + \gamma \frac{\tan{\alpha'}+ v/u_0^{x}}{1+\tan{\alpha'}u_0^{x}v}}|
\end{equation}




\end{document}