\documentclass{article}
\usepackage[utf8]{inputenc}
\usepackage{amsmath}
\usepackage{amssymb}
\usepackage{physics}
\usepackage{gensymb}
\usepackage{esvect}
\usepackage[title]{appendix} % or other options
\usepackage{graphicx} % Required for inserting images

% Custom commands for partial derivatives
\newcommand{\pd}{\partial}  % Short for \partial
\newcommand{\pdm}{\partial_\mu}  % \partial_\mu
\newcommand{\pdn}{\partial_\nu}  % \partial_\nu
\newcommand{\pdup}{\partial^\mu}  % \partial^\mu
\newcommand{\pdupnu}{\partial^\nu}  % \partial^\nu
\newcommand{\Lag}{\mathcal{L}}  % Lagrangian shorthand
\newcommand{\onehalf}{\frac{1}{2}}

% Alternative shorter versions
\newcommand{\dmu}{\partial_\mu}
\newcommand{\dnu}{\partial_\nu}
\newcommand{\dmuup}{\partial^\mu}
\newcommand{\dnuup}{\partial^\nu}

% Even shorter versions (if you prefer)
\newcommand{\dm}{\partial_\mu}
\newcommand{\dn}{\partial_\nu}
\newcommand{\dmuu}{\partial^\mu}
\newcommand{\dnuu}{\partial^\nu}

\title{Personal Solutions to Problem Sheet 1 QFT by David Tong}
\author{Baset}
\date{June 2025}

\begin{document}

\maketitle
\section*{1.}
According to Eq. (2),
\begin{equation}
    \begin{split}
        \frac{\partial y}{\partial t} &= \sqrt{\frac{2}{a}}\sum_{n=1}^\infty \sin(\frac{n\pi x}{a})\dot{q}_n\\
        \frac{\partial y}{\partial x} &= \sqrt{\frac{2}{a}}\sum_{n=1}^\infty \cos(\frac{n\pi x}{a})\frac{n\pi}{a}q_n
    \end{split}
\end{equation}
implying (assuming the integrals are finite and convergent, $m,n > 0$):
\begin{equation}
    \begin{split}
        L &= \int_0^a dx \left[\frac{\sigma}{2}\frac{2}{a}\left(\sum_{n=1}^\infty \sin\left(\frac{n\pi x}{a}\right)\dot{q}_n\right)^2 - \frac{T}{2}\frac{2}{a}\left(\sum_{n=1}^\infty \cos\left(\frac{n\pi x}{a}\right)\frac{n\pi}{a}q_n\right)^2 \right]\\
          &=\frac{1}{a}\int_0^a dx\left[\sigma \sum_{m,n}\sin(\frac{n\pi}{a}x)\sin(\frac{m\pi}{a}x)\dot{q}_n\dot{q}_m-T\sum_{m,n}\cos(\frac{n\pi}{a}x)\cos(\frac{m\pi}{a}x)(\frac{\pi}{a})^2 \, mn\, q_nq_m  \right] \\
          &= \frac{1}{a}\sum_{m,n}\int_0^a dx \left[\sigma \frac{\cos((m-n)\frac{\pi}{a}x)-\cos((m+n)\frac{\pi}{a}x)}{2}\dot{q}_n\dot{q}_m - T \frac{\cos((m-n)\frac{\pi}{a}x)+\cos((m+n)\frac{\pi}{a}x)}{2}\right.\\
          &\left.\quad(\frac{\pi}{a})^2 \, mn\, q_nq_m \right] = \frac{1}{a}\sum_{m,n} \left[ \frac{\sigma}{2}\delta_{m,n}\dot{q}_n\dot{q}_m - (\frac{\pi}{a})^2 \delta_{m,n} \, mn\, q_nq_m \frac{T}{2} \right] \\
          &= \sum_{n=1}^\infty \left[ \frac{\sigma}{2}\dot{q}_n^2 - \frac{T}{2}(\frac{n\pi}{a})^2 q_n^2  \right] = L(q_n,\dot{q}_n)  
        \end{split}
\end{equation}
E-L equations imply:

\begin{equation}
    \begin{split}
       & -\frac{\partial L}{\partial q_n} + \partial_\mu \frac{\partial L}{\partial_\mu(q_n)} = 0 \quad \equiv T(\frac{n\pi}{a})^2q_n + \sigma \ddot{q}_n = 0 \implies \\
       & \ddot{q}_n + \frac{T}{\sigma}(\frac{n\pi}{a})^2 q_n = 0 \implies \omega_n = \sqrt{\frac{T}{\sigma}} (\frac{n\pi}{a})\\
    \end{split}
\end{equation}


\section*{2.}
According to the notation in the notes $\phi'(x) = \phi(y)$, implying
\begin{equation}
    y^\nu = (\Lambda^{-1})_\mu^\nu x^\mu \implies \frac{\partial y^\nu}{\partial x^\mu} = (\Lambda^{-1})_\mu^\nu
\end{equation}
The KG in the notes is $\partial_\mu \partial^\mu \phi(x) + m^2 \phi(x) = 0$, the KG in the new 
coordinate system:
\begin{equation}
    \begin{split}
       \text{KG}': &(\Lambda^{-1})^\mu_\nu \partial_\mu (\Lambda^{-1})_\mu^\nu \partial^\mu \phi(y) + m^2 \phi(y) = 0\\
        & \equiv \partial_\nu \partial^\nu \phi(y) + m^2\phi(y) = 0  
    \end{split}
\end{equation}

\section*{3.}
E-L equations:
\begin{equation}
    \begin{cases}
         \text{Eq1: }& \pdm \frac{\pd \Lag}{\pd (\pdm \psi^*)} - \frac{\pd \Lag}{\pd \psi^*} = 0\\
         \text{Eq2: }& \pdm \frac{\pd \Lag}{\pd (\pdm \psi)} - \frac{\pd \Lag}{\pd \psi} = 0
    \end{cases}
    \implies 
    \begin{cases}
        \text{- }& \pdm \pdup \psi + m^2 \psi + \lambda \psi^*\psi^2 = 0 \\
        \text{- }& \pdm \pdup \psi^* + m^2 \psi^* + \lambda \psi(\psi^*)^2 = 0 
    \end{cases}
\end{equation}
The invariance part and the changed Lagrangian up to the first order:
\begin{equation}
    \begin{split}
    \Lag' & \simeq \pdm (\psi^* -i\alpha\psi^*) \pdup (\psi + i\alpha\psi)-m^2\psi^*\psi -\frac{\lambda}{2}(\psi^*\psi)^2 \\
        & \simeq \pdm\psi^* \pdup\psi -m^2\psi^*\psi -\frac{\lambda}{2}(\psi^*\psi)^2 = \Lag
    \end{split} 
\end{equation}
therefore, the conserved current is:
\begin{equation}
    \begin{split}
    j^\mu = &\frac{\pd \Lag }{\pd (\pdm\phi_a)}X_a(\phi) = i\alpha\psi\pdup\psi^* - i\alpha\psi^*\pdup\psi \\
    & \equiv i(\psi\pdup\psi^* - \psi^*\pdup\psi)
    \end{split}
\end{equation}
We calculate explicitly $\pdm j^\mu$ and use the E-L:
\begin{equation}
    \begin{split}
        \pdm j^\mu & = i\left[ \pdm\psi\pdup\psi^* + \psi\pdm\pdup\psi^* - \pdm\psi^* \pdup\psi - \psi^* \pdm\pdup\psi \right]\\
        & = i\left[ -\psi\left(m^2\psi^* + \lambda\psi (\psi^*)^2 \right) + \psi^*(m^2\psi + \lambda\psi^*\psi^2) \right] \\
        & = 0
    \end{split}
\end{equation}
QED.

\section*{4.}
\begin{equation}
    \Lag = \onehalf\pdm \phi_a \pdup \phi_a - \onehalf m^2 \phi_a\phi_a \implies 
\end{equation}

\begin{equation}
    \begin{split}
        \Lag' & \simeq \onehalf\pdm(\phi_a + \theta\epsilon_{abc}n_b\phi_c)\pdup (\phi_a + \theta\epsilon_{abc}n_b\phi_c)-
        \onehalf m^2 (\phi_a\phi_a - 2\theta \epsilon_{bac}\phi_a\phi_c)\\
        & \simeq \onehalf \{\pdm \phi_a \pdup\phi_a + \theta n_b \left[\epsilon_{abc}\pdm\phi_c \pdup\phi_a 
        + \epsilon_{abc}\pdup\phi_c \pdm\phi_a  \right]  \} - \onehalf m^2 \phi_a\phi_a \\
        & = \onehalf\pdm \phi_a \pdup \phi_a - \onehalf m^2 \phi_a\phi_a = \Lag
    \end{split}
\end{equation}
We used the fact that $\epsilon_{abc}$ tensor is anti-symmetric, but $\pdm\phi_c \pdup\phi_a$ is symmetric w.r.t
changing the indices $a$ and $c$. The same goes for $\phi_a\phi_c$.

Computing the Noether current:
\begin{equation}
    \begin{split}
        j^\mu & = \frac{\pd\Lag}{\pd(\pdm \phi_a)}X_a(\phi) \\
        & = \pdup\phi_a \, \epsilon_{abc}n_b\phi_c \implies \\
        Q & = \int d^3x \, \epsilon_{abc} \dot{\phi_a} n_b \phi_c \\
        & =  n_b \int d^3x \,\epsilon_{bca} \dot{\phi_a} \phi_c \\ 
        & = n_b \int d^3x \, \epsilon_{bac} \dot{\phi_c} \phi_a = n_a \int d^3x \, 
        \epsilon_{abc} \dot{\phi_b} \phi_c 
    \end{split}
\end{equation}
We can choose $n_a = (1,0,0)$, then for each choice:
\begin{equation}
    Q_a = \int d^3x \, 
    \epsilon_{abc} \dot{\phi_b} \phi_c 
\end{equation}
Direct confirmation:
\begin{equation}
    \begin{split}
        \Lag & = \onehalf\pd_t\phi_a\pd_t\phi_a - \onehalf\nabla \phi_a\nabla\phi_a-\onehalf m^2\phi_a\phi_a \implies \\
        \text{E-L for each $a$: } & \pd_t^2 \phi_a - \nabla^2\phi_a + m^2\phi_a = 0 
    \end{split}
\end{equation} 
Hence:
\begin{equation}
    \begin{split}
        \frac{d \, Q_a}{dt} & = \int d^3x \, \epsilon_{abc}\ddot{\phi_a}\phi_c + \int  
        d^3x \, \epsilon_{abc}\dot{\phi_a}\dot{\phi_c}  \\
        & = \int d^3x \, \epsilon_{abc}(\nabla^2 \phi_a - m^2\phi_a)\phi_c = 
         \int d^3x \, \epsilon_{abc} \nabla^2 \phi_a \, \phi_c \\
         & = - \int d^3x \, \epsilon_{abc} \nabla\phi_a.\nabla\phi_c = 0
    \end{split}
\end{equation}
We have used the symmetric, anti-symmetric point several times in the above derivation.


\section*{5.}
- The first result is:
\begin{equation}
    \begin{split}
    \eta_{\sigma\tau}x'^\sigma x'^{\tau} & = \eta_{\sigma\tau}\Lambda_\mu^\sigma \, x^\mu \Lambda^\tau_\nu \, x^\nu = \eta_{\mu\nu}x^\mu x^\nu \implies \\
    \eta_{\mu\nu} & = \eta_{\sigma\tau}\Lambda_\mu^\sigma \Lambda^\tau_\nu
    \end{split}
\end{equation}

For any transformation to be Lorentz, it must satisfy Eq.(16):
\begin{equation}
    \begin{split}
        \eta_{\mu\nu} & = \eta_{\sigma\tau}(\delta^\sigma_\mu + \omega^\sigma_\mu)(\delta^\tau_\nu + \omega^\tau_\nu)\\
        \eta_{\mu\nu} & = \eta_{\mu\nu} + \eta_{\mu\tau} \omega^\tau_\nu + \eta_{\sigma\nu}\omega^\sigma_\mu + \eta_{\sigma\tau}\omega^\sigma_\mu\omega^\tau_\nu \\
        & \simeq \eta_{\mu\nu} + (\omega_{\mu\nu} + \omega_{\nu\mu}) 
    \end{split}
\end{equation}
Hence:
\begin{equation}
    \omega^{\mu\nu} = - \omega^{\nu\mu}
\end{equation}
A pure rotation:
\begin{equation}
    \begin{split}
    R(\theta) & = \begin{bmatrix}
            1 & 0 & 0 & 0 \\
            0 & \cos{\theta} & -\sin{\theta} & 0 \\
            0 & \sin{\theta} & \cos{\theta} & 0 \\ 
            0 & 0 & 0 & 1
                \end{bmatrix} \\
    & \simeq \begin{bmatrix}
            1  & 0 & 0 & 0 \\
            0  & 1 & -\theta & 0\\
            0 & \theta & 1 & 0 \\
            0 & 0 & 0 & 1  
            \end{bmatrix} = [\delta] + \begin{bmatrix}
                0  & 0 & 0 & 0 \\
                0  & 0 & \theta & 0\\
                0 & -\theta & 0 & 0\\
                0 & 0 & 0 & 0
            \end{bmatrix}
    \end{split}
\end{equation}
Anti-symmetric as one can see for $\theta \ll 1$ infinitesimally small.
In cas of the boost:
\begin{equation}
    \begin{split}
        \Lambda(v) & = \begin{bmatrix}
                \gamma & -\gamma v & 0 & 0\\
                -\gamma v & \gamma & 0 & 0 \\
                0 & 0 & 1 & 0 \\
                0 & 0 & 0 & 1
                        \end{bmatrix}
    \end{split}
\end{equation}
$\gamma(v) \simeq 1 + \onehalf v^2 \implies $
\begin{equation}
    \begin{split}
        \Lambda(v) & \simeq \begin{bmatrix}
             1 & - v & 0 & 0\\
                -v & 1 & 0 & 0 \\
                0 & 0 & 1 & 0 \\
                0 & 0 & 0 & 1
                        \end{bmatrix} = [\delta] + \begin{bmatrix}
                            0 & - v & 0 & 0\\
                               -v & 0 & 0 & 0 \\
                               0 & 0 & 0 & 0 \\
                               0 & 0 & 0 & 0
                                       \end{bmatrix}
    \end{split}
\end{equation}
Which will be antisymmetric after we lower the index using Minkowski metric.
\section*{6.}
\begin{equation}
    \phi(x) \xrightarrow{} \phi'(x') = \phi(x^\mu - \omega^\mu_\nu x^\nu) \simeq \phi(x) - \omega^\mu_\nu x^\nu \pdm \phi
\end{equation}
Therefore:
\begin{equation}
    \Lag'(\phi') = \Lag(\phi-\omega^\mu_\nu x^\nu \pdm \phi) \implies \delta\Lag = -\omega^\mu_\nu x^\nu \pdm \Lag 
\end{equation}
Which because $\omega$ is infinitesimal and antisymmetric:
\begin{equation}
    \delta\Lag = - \pdm (\omega^\mu_\nu x^\nu \Lag)
\end{equation}
Using Noether's theorem:
\begin{equation}
    \begin{split}
        j^\mu &= -\frac{\pd\Lag}{\pd (\pdm \phi)}\omega^\rho_\nu x^\nu \pd_{\rho} \phi + \omega^\mu_\nu x^\nu \Lag \\
        & = -\omega^\rho_\nu \left[ \frac{\pd\Lag}{\pd (\pdm \phi)} x^\nu \pd_{\rho} \phi - \delta^\mu_\rho\Lag x^\nu \right]\\
        & = -\omega^\rho_\nu \left[ T_\rho^\mu x^\nu \right]
    \end{split}
\end{equation}
Accordingly, looking at Eq. (19), for arbitrary $j\ne k$, $\omega_{jk}=-\omega_{kj}$, hence:
\begin{equation}
    \begin{split}
        Q &= -\int d^3x \, T^{\rho 0}\omega_{\rho\nu}x^\nu = -\int d^3x \, (T^{j 0}\omega_{jk}x^k -T^{k0} \omega_{jk}x^j) \\
    \end{split}
\end{equation}
We can write the above equation for three pairs, and also we have a freedome in choosing $\omega_{jk}=\pm 1$, therefore 
using Levi-Civita symbol:
\begin{equation}
    Q_i = \epsilon_{ijk} \int d^3x \, (x^jT^{0k} - x^kT^{0j})
\end{equation}
Which is just the Angular momentum.
The other one resulting from the Lorentz Boosts is:
\begin{equation}
    \begin{split}
        Q &= \int d^3x (x^iT^{00} - x^0T^{0i}) \implies \frac{d\,Q}{dt} = 0 \implies \\
        & \frac{d}{dt}\int d^3x \, x^iT^{00} = \int d^3x \, T^{0i}  = P^i
    \end{split}
\end{equation}
My own first impression was that this is sort of a restatement of Newton's law and sort of restatement
for what momentum is, but a more precise answer in the book correctly says that this equation states 
that the center of energy's velocity is constant, or just the momentum we have defined which in 
translation invariant systems must be preserved.

\section*{7.}
For the first part we only prove that the $F_{\mu\nu}$ tensor is invariant under the Guage the transformation
introduced here:
\begin{equation}
    \begin{split}
        F'_{\mu\nu} & = (\pdm A'_\nu - \pdn A'_\mu) = \pdm A_\nu - \pdn A_\mu + \pdn \pdm \xi - \pdm\pdn \xi = F_{\mu\nu}
    \end{split}
\end{equation}
Therefore the Lagrangian does not change under Guage transformation.

For the translation trans formation we follow the note's explanation for deriving the energy-momentum tensor,
$x^\nu \xrightarrow{} x^\nu - \epsilon^\nu$, hence: $A_\nu \xrightarrow{} A_\nu + \epsilon^\mu \pdm A_\nu $,
 therefore the energy-momentum tensor is:
 \begin{equation}
    \begin{split}
        T^\mu_\nu &= \frac{\pd\Lag}{\pd (\pdm A_\rho)}\pdn A_\rho - \delta^\mu_\nu \Lag = -F^{\mu\rho}\pdn A_\rho - \delta^\mu_\nu \Lag \implies \\
        T^{\mu\nu} & = -F^{\mu\rho}\pdupnu A_\rho - \eta^{\mu\nu}\Lag
    \end{split}
 \end{equation}
All the terms above except for $\pdupnu A_\rho$ are Guage invariant. But, obviously the term mentioned isn't and therefore
the obtained $T^{\mu\nu}$ can not be Guage invariant. Moreover, the excluding the Lagrangian term of the 
energy-momentum tensor, it can not be symmetric w.r.t. $\mu$ and $\nu$, one can easily compute $(0,1)$ term and 
$(1,0)$ term to see the tensor not being symmetric.
Now we investigate the proposed tensor:
\begin{equation}
    \Theta^{\mu\nu} = T^{\mu\nu}-F^{\rho\mu}\pd_{\rho}A^\nu
\end{equation}
Using Eq.(30):
\begin{equation}
    \begin{split}
        \Theta^{\mu\nu} &= -F^{\mu\rho}\pdupnu A_\rho - \eta^{\mu\nu}\Lag + F^{\mu\rho}\pd_\rho A^\nu \\
        & = F^{\mu\rho}(\pd_\rho A^\nu - \pdupnu A_\rho) - \eta^{\mu\nu}\Lag \\
        & = F^{\mu\rho}\eta^{\nu\sigma}(\pd_\rho A_\sigma - \pd_\sigma A_\rho) - \eta^{\mu\nu}\Lag \\
        & = F^{\mu\rho}F_{\rho\sigma}\eta^{\nu\sigma} - \eta^{\mu\nu}\Lag 
    \end{split}
\end{equation}
Before confirming the conserved currents we see that it is completely Guage invariant and also Symmetric.

The E-L equations according to the Lagrangian are: $\pdm F^{\mu\nu} = 0$, for the currents:
\begin{equation}
    \begin{split}
        \pdm \Theta^{\mu\nu} & = \eta^{\sigma\nu}F_{\rho\sigma}\pdm F^{\mu\rho} + \eta^{\sigma\nu}F^{\mu\rho}\pdm F_{\rho\sigma}+\frac{1}{2}\eta^{\mu\nu}F^{\rho\sigma}\pdm F_{\rho\sigma}\\
        & = \{ \text{$\mu \leftrightarrow \sigma $}\}= 0 + \eta^{\mu\nu}F^{\sigma\rho}\pd_\sigma F_{\rho\mu} + \onehalf 
        \eta^{\mu\nu}F^{\rho\sigma}\pdm F_{\rho\sigma} \\
        & = \eta^{\mu\nu}F^{\sigma\rho} \left\{\pd_\sigma F_{\rho\mu} - \onehalf \pdm F_{\rho\sigma} \right\} \\
        & = \eta^{\mu\nu}F^{\sigma\rho} \left\{A_{\mu,\rho\sigma} - A_{\rho,\mu\sigma} - \onehalf A_{\sigma,\rho\mu} + \onehalf A_{\rho,\sigma\mu}  \right\} \\
        & = \onehalf \eta^{\mu\nu}F^{\sigma\rho} \left\{ A_{\mu,\rho\sigma} - A_{\rho,\mu\sigma} +  A_{\mu,\rho\sigma} - A_{\sigma,\rho\mu} \right\} \\
        & = \onehalf \eta^{\mu\nu}F^{\sigma\rho} \left\{ \pd_\sigma F_{\rho\mu} - \pd_\rho F_{\mu\sigma} \right\} = -
        \onehalf \eta^{\mu\nu} \left\{ F^{\sigma\rho}\pd_{\sigma}F_{\mu\rho} + F^{\sigma\rho}\pd_{\rho}F_{\mu\sigma} \right\}\\
        & = -\onehalf \eta^{\mu\nu} \left\{ F^{\sigma\rho} \pd_{\rho} F_{\mu\sigma} - F^{\rho\sigma}\pd_\sigma F_{\mu\rho}  \right\} = \{ \text{$\rho \leftrightarrow \sigma $}\}= \\
        & = -\onehalf \eta^{\mu\nu} \left\{ 0 \right\} = 0
    \end{split}
\end{equation}
Therefore this also defines four conserved currents. For the traceless proof:
\begin{equation}
    \Theta^\mu_\mu = -F^{\mu\rho}F_{\mu\rho} - \eta^{\mu}_\mu \Lag = 4\Lag - 4\Lag = 0
\end{equation}

\section*{8.}
We use the $E-L$ equation for fields:
\begin{equation}
    \begin{split}
        0 &= -\pdm \frac{\pd\Lag}{\pd(\pdm C_\nu)} + \frac{\pd\Lag}{\pd C_\nu} = \pdm F^{\mu\nu} + m^2C^\nu \\
        & = (\pdm\pdup + m^2)C^\nu - \pdupnu \pdm C^\mu   
    \end{split}
\end{equation}
We have:
\begin{equation}
    \begin{split}
        m^2C^\nu &= \pdupnu \pdm C^\mu - \pdm\pdup C^\nu \implies m^2 \pdn C^\nu = \pdn\pdupnu\pdm C^\mu - 
        \pdm\pdup\pdn C^\nu = 0 \\
        & \implies m^2 \pdm C^\mu = 0 \xrightarrow{m \ne 0} \pdm C^\mu = 0
    \end{split}
\end{equation}
This, by itself helps to write one of the components based on the other (E-L, $\nu = 0$):
\begin{equation}
    \begin{split}
       & \pd_t^2 C^0 + (m^2 + \pd_i\pd^i)C^0 - \pd_t^2 C^0 - \pd^i \dot{C}_i = 0 \implies \\
       & (m^2 + \pd_i\pd^i)C^0 =  \pd^i \dot{C}_i
    \end{split}
\end{equation}
By definition:
\begin{equation}
    \begin{split}
        \Pi^i &= \frac{\pd \Lag}{\pd \dot{C}_i} = -F^{0i} \implies \Pi^0 = -F^{00} = 0 
    \end{split}
\end{equation}
Then the Hamiltonian density:
\begin{equation}
    \begin{split}
        \mathcal{H} & = \Pi^i \dot{C}_i - \Lag = \Pi^i(F_{0i}+\pd_iC_0)-\Lag = -\Pi^i\Pi_i + \Pi^i\pd_iC_0 + \onehalf \Pi^i\Pi_i + \onehalf F^{ij}F_{ij}\\
        &-\onehalf m^2 C_0C^0 - \onehalf m^2 C_iC^i \implies \\
        \mathcal{H} & = \onehalf(\Pi_i)^2 - \Pi_i\pd_iC_0 + \onehalf F^{ij}F_{ij} - \onehalf m^2 C_0^2 + \onehalf m^2 C_i^2
    \end{split}
\end{equation}
\end{document}
